examples.v
@@ -1,0 +1,194 @@
+Require Export lang.
+Require Export ISL.
+
+(* in this example v is a (EVal (VLoc n))
+   describing in the location in the heap where
+   we will find a second location. In C parlance
+   this would be a
+   v ** int so a pointer to a vector of integers.
+
+   In our case the underlying vector is just one cell
+   so we can free and allocate just one to simulate
+   a use after free bug later on.
+ *)
+
+ Definition push_back : expr → expr :=
+  fun v =>
+    (ELet "z" EAmb
+          (EIf (EOp EqOp (EVar "z") (EVal (VNat 0)))
+               (EVal VUnit)
+               (ELet "y" (ELoad v) (* now y points to the underlying array *)
+                     (ESeq (EFree (EVar "y"))
+                           (ELet "y" (EAlloc (EVal (VNat 42)))
+                                 (EStore v (EVar "y"))))))).
+
+Example example_push_back := push_back (EVal (VLoc 0)).
+Check example_push_back.
+Print example_push_back.
+Compute example_push_back.
+
+(* client is where we will trigger the use-after-free
+   error as we get a hold of a location that might be
+   deallocated
+ *)
+Definition client : expr :=
+    (ELet "w" (EAlloc (EVal (VNat 0)))
+          (ELet "v" (EAlloc (EVar "w"))
+
+    (ELet "x" (ELoad (EVar "v"))
+          (ESeq (push_back (EVar "v")) (* here the underlying storage for v might be moved *)
+                (EStore (EVar "x") (EVal (VNat 88))))))). (* so using the previous location might fault *)
+
+
+
+Lemma client_can_error : will_error iEmpty client.
+Proof.
+  unfold will_error, client.
+  exists empty.
+  (* {[ 0 := (VNat 0) ]} ∪ {[ 1 := (VLoc 0) ]} ∪ {[ 2 := (VNat 42) ]}. *)
+  exists ({[ 0 := Reserved ]} ∪ {[ 1 := (Value (VLoc 2)) ]} ∪ {[ 2 := (Value (VNat 42)) ]}).
+  exists (EStore (EVal (VLoc 0)) (EVal (VNat 88))).
+  split; [done |].
+  split.
+  - eapply steps_trans.
+    eapply steps_let_val'.
+    + apply steps_single.
+      apply (Alloc_headstep ∅ (VNat 0) 0).
+      unfold valid_alloc.
+      intros e H.
+      exfalso.
+      eapply lookup_empty_is_Some.
+      eexists e.
+      eauto.
+    + rewrite insert_empty.
+      simpl subst.
+      eapply steps_trans.
+      eapply steps_let_val'.
+      * apply steps_single.
+        apply (Alloc_headstep {[0:= (Value (VNat 0))]} (VLoc 0) 1).
+        unfold valid_alloc.
+        rewrite lookup_singleton_ne.
+        discriminate.
+        auto.
+      * simpl subst.
+        rewrite insert_union_singleton_l.
+        eapply steps_trans.
+        eapply steps_let_val'.
+        -- apply steps_single.
+           econstructor.
+           eapply lookup_union_Some; auto.
+           rewrite map_disjoint_singleton_l. auto using lookup_singleton_None.
+        -- simpl subst.
+           eapply steps_seq_val'.
+           ++ eapply steps_trans.
+              eapply steps_let_val'.
+              ** apply steps_single.
+                 apply (Amb_headstep ({[1 := (Value (VLoc 0))]} ∪ {[0 := (Value (VNat 0))]}) 1).
+              ** simpl subst.
+                 eapply steps_trans.
+                 apply steps_if_false'.
+                 --- eauto using steps_single, head_step.
+                 --- eapply steps_trans. apply steps_let_val'.
+                     +++ eauto using steps_single, head_step.
+                     +++ simpl subst.
+                         eapply steps_seq_val'.
+                         *** eauto using steps_single, head_step.
+                         *** eapply steps_trans.
+                             ---- apply steps_let_val'.
+                                  apply steps_single.
+                                  rewrite insert_union_r.
+                                  rewrite insert_singleton.
+                                  apply (Alloc_headstep ({[1 := Value (VLoc 0)]} ∪ {[0 := Reserved]}) (VNat 42) 2).
+                                  unfold valid_alloc.
+                                  intros.
+                                  erewrite lookup_union_Some in H.
+                                  destruct H as [H | H]; rewrite lookup_singleton_ne in H; discriminate.
+                                  solve_map_disjoint.
+                                  auto using lookup_singleton_ne.
+                             ---- simpl subst.
+                                  apply steps_single.
+                                  eauto using head_step.
+           ++ rewrite insert_commute; eauto.
+              rewrite insert_union_l.
+              rewrite insert_union_singleton_r.
+              rewrite insert_singleton.
+              assert (
+                  ({[1 := Value (VLoc 2)]} ∪ {[0 := Reserved]} : mem)
+                  =
+                  ({[0 := Reserved]} ∪ {[1 := Value (VLoc 2)]})
+              ).
+              { admit. }
+              assert (
+                  ({[1 := Value (VLoc 2)]} ∪ {[0 := Reserved]} ∪ {[2 := Value (VNat 42)]}: mem)
+                  =
+                  ({[0 := Reserved]} ∪ {[1 := Value (VLoc 2)]} ∪ {[2 := Value (VNat 42)]})
+              ).
+              { admit. }
+              rewrite H0.
+              apply steps_refl.
+              rewrite lookup_union_None.
+              split; simpl_map; reflexivity.
+  - unfold is_error.
+    split.
+    + auto.
+    + intros.
+      intro.
+      erewrite step_store_inv in H. destruct H as (w & lookup_h & _ & _).
+      do 2 erewrite lookup_union_Some in lookup_h.
+      destruct lookup_h as [ [a|b] | c].
+      * rewrite lookup_singleton in a.
+        discriminate.
+      * rewrite lookup_singleton_ne in b.
+        discriminate.
+        auto.
+      * rewrite lookup_singleton_ne in c.
+        discriminate.
+        auto.
+      * solve_map_disjoint.
+      * solve_map_disjoint.
+      * solve_map_disjoint.
+Admitted.
+
+
+(* now this example may error if the test evaluates to true *)
+Example may_error := (EIf amb_bool EError (EVal VUnit)).
+
+Lemma may_error_contains_error : ∀ m,  contains_error may_error m.
+Proof.
+  unfold contains_error, may_error, amb_bool.
+  intros.
+  eexists EError, m.
+  split.
+  - apply (steps_step
+             m m m
+             (EIf (EOp EqOp EAmb (EVal (VNat 0))) EError (EVal VUnit))
+             (EIf (EOp EqOp (EVal (VNat 0)) (EVal (VNat 0))) EError (EVal VUnit))).
+    + change (EIf (EOp EqOp EAmb (EVal (VNat 0))) EError (EVal VUnit)) with
+          (fill [(IfCtx EError (EVal VUnit)); (OpCtxL EqOp (EVal (VNat 0)))] EAmb).
+      change (EIf (EOp EqOp (EVal (VNat 0)) (EVal (VNat 0))) EError (EVal VUnit)) with
+          (fill [(IfCtx EError (EVal VUnit)); (OpCtxL EqOp (EVal (VNat 0)))] (EVal (VNat 0))).
+      constructor.
+      constructor.
+    + apply (steps_step
+             m m m
+             (EIf (EOp EqOp (EVal (VNat 0)) (EVal (VNat 0))) EError (EVal VUnit))
+             (EIf (EVal (VBool true)) EError (EVal VUnit))).
+      * change (EIf (EOp EqOp (EVal (VNat 0)) (EVal (VNat 0))) EError (EVal VUnit)) with
+            (fill [(IfCtx EError (EVal VUnit))] (EOp EqOp (EVal (VNat 0)) (EVal (VNat 0)))).
+        change (EIf (EVal (VBool true)) EError (EVal VUnit)) with
+            (fill [(IfCtx EError (EVal VUnit))] (EVal (VBool true))).
+        constructor.
+        constructor.
+        simpl.
+        reflexivity.
+      * apply steps_if_true.
+  - unfold is_error.
+    split; auto.
+    intros.
+    intro.
+    inversion H.
+    destruct E; simpl in *.
+    + subst.
+      inversion H1.
+    + destruct c; simpl in *; discriminate || auto.
+Qed.
